Prove rePEG wfG
Required adding a rule for CharSet. This rule could use improvement.

The methodolgy for proving wfG is not completely clear. But it seems
like there should be a library for doing this more generally, to save
PEG users pain.

examples/formal-languages/regular/regexp_parserScript.sml
@@ -1,6 +1,6 @@
 open HolKernel Parse boolLib bossLib;
 
-open regexpTheory pegTheory monadsyntax
+open regexpTheory pegTheory pegexecTheory monadsyntax
 
 val _ = new_theory "regexp_parser";
 
@@ -80,6 +80,19 @@ val OrM_def = Define‘
   OrM roptlist = OPTION_MAP Or (OPT_MMAP I roptlist)
 ’
 
+(* breaks abstraction, see TODO on mkNT Charset below *)
+val charset_char_def = Define`
+  charset_char c = Chset (Charset (n2w (ORD c)) 0w 0w 0w)`;
+val uncharset_char_def = Define`
+  (uncharset_char (Chset (Charset w _ _ _)) = CHR (w2n w)) ∧
+  (uncharset_char _ = CHR 0)`;
+val uncharset_char_charset_char = Q.store_thm("uncharset_char_charset_char[simp]",
+  `uncharset_char (charset_char c) = c`,
+  rw[charset_char_def,uncharset_char_def]
+  \\ srw_tac[wordsLib.WORD_ss][]
+  \\ qspec_then`c`strip_assume_tac stringTheory.ORD_BOUND
+  \\ rw[stringTheory.CHR_ORD]);
+
 val rePEG_def = Define‘
   rePEG = <|
     start := pnt Top ;
@@ -103,6 +116,14 @@ val rePEG_def = Define‘
          tok ((=) #"d") (K (SOME (Chset DigitSet)));
          tok EscapableChar (λcl. SOME (Chset (charset_sing (FST cl))))
        ]);
+
+      (mkNT CharSet,
+       (* TODO: add complement, ranges, escaped chars, etc. *)
+       (* TODO: this might be better if we weren't forced into the regexp type
+       (so could accumulate the list of characters easier), maybe use a sum? *)
+       rpt (tok ((<>) #"]") (λcl. SOME (charset_char (FST cl))))
+         (λls. OPTION_MAP (Chset o charset_string)
+                 (OPT_MMAP (OPTION_MAP uncharset_char) ls)));
 
       (mkNT Star,
        seq (pnt Atom) (try (tok ((=) #"*") (K (SOME (Chset charset_empty)))))
@@ -133,9 +154,104 @@ val rePEG_def = Define‘
   |>
 ’;
 
+val FDOM_rePEG = save_thm("FDOM_rePEG",
+  EVAL``FDOM rePEG.rules``);
+
+val wfpeg_BslashSpecial_applied = Q.store_thm("wfpeg_BslashSpecial_applied",
+  `wfpeg rePEG (rePEG.rules ' (mkNT BslashSpecial))`,
+  CONV_TAC(RAND_CONV EVAL)
+  \\ rpt(rw[Once wfpeg_cases]));
+
+val wfpeg_BslashSpecial = Q.store_thm("wfpeg_BslashSpecial",
+  `wfpeg rePEG (nt (mkNT BslashSpecial) I)`,
+  rw[Once wfpeg_cases] >- EVAL_TAC
+  \\ rw[wfpeg_BslashSpecial_applied]);
+
+val wfpeg_CharSet_applied = Q.store_thm("wfpeg_CharSet_applied",
+  `wfpeg rePEG (rePEG.rules ' (mkNT CharSet))`,
+  CONV_TAC(RAND_CONV EVAL)
+  \\ ntac 2 (rw[Once wfpeg_cases]));
+
+val wfpeg_CharSet = Q.store_thm("wfpeg_CharSet",
+  `wfpeg rePEG (nt (mkNT CharSet) I)`,
+  rw[Once wfpeg_cases] >- EVAL_TAC
+  \\ rw[wfpeg_CharSet_applied]);
+
+val wfpeg_Atom_applied = Q.store_thm("wfpeg_Atom_applied",
+  `wfpeg rePEG (rePEG.rules ' (mkNT Atom))`,
+  CONV_TAC(RAND_CONV EVAL)
+  \\ rpt(rw[Once wfpeg_cases]));
+
+val wfpeg_Atom = Q.store_thm("wfpeg_Atom",
+  `wfpeg rePEG (nt (mkNT Atom) I)`,
+  rw[Once wfpeg_cases] >- EVAL_TAC
+  \\ rw[wfpeg_Atom_applied]);
+
+val wfpeg_Star_applied = Q.store_thm("wfpeg_Star_applied",
+  `wfpeg rePEG (rePEG.rules ' (mkNT Star))`,
+  CONV_TAC(RAND_CONV EVAL)
+  \\ rw[Once wfpeg_cases,wfpeg_Atom]
+  \\ rpt(rw[Once wfpeg_cases]));
+
+val wfpeg_Star = Q.store_thm("wfpeg_Star",
+  `wfpeg rePEG (nt (mkNT Star) I)`,
+  rw[Once wfpeg_cases] >- EVAL_TAC
+  \\ rw[wfpeg_Star_applied])
+
+val wfpeg_Concat_applied = Q.store_thm("wfpeg_Concat_applied",
+  `wfpeg rePEG (rePEG.rules ' (mkNT Concat))`,
+  CONV_TAC(RAND_CONV EVAL)
+  \\ rw[Once wfpeg_cases]
+  >- rw[wfpeg_Star]
+  \\ fs[Once peg0_cases]
+  \\ fs[EVAL``rePEG.rules ' (mkNT Star)``]
+  \\ fs[Once peg0_cases]
+  \\ fs[Once peg0_cases]
+  \\ fs[EVAL``rePEG.rules ' (mkNT Atom)``]
+  \\ rw[] \\ fs[]
+  \\ fs[Once peg0_cases]);
+
+val wfpeg_Concat = Q.store_thm("wfpeg_Concat",
+  `wfpeg rePEG (nt (mkNT Concat) I)`,
+  rw[Once wfpeg_cases] >- EVAL_TAC
+  \\ rw[wfpeg_Concat_applied]);
+
+val wfpeg_Alt_applied = Q.store_thm("wfpeg_Alt_applied",
+  `wfpeg rePEG (rePEG.rules ' (mkNT Alt))`,
+  CONV_TAC(RAND_CONV EVAL)
+  \\ rw[Once wfpeg_cases,wfpeg_Concat]
+  \\ ntac 3 (rw[Once wfpeg_cases]));
+
+val wfpeg_Alt = Q.store_thm("wfpeg_Alt",
+  `wfpeg rePEG (nt (mkNT Alt) I)`,
+  rw[Once wfpeg_cases] >- EVAL_TAC
+  \\ rw[wfpeg_Alt_applied]);
+
+val wfpeg_Top_applied = Q.store_thm("wfpeg_Top_applied",
+  `wfpeg rePEG (rePEG.rules ' (mkNT Top))`,
+  CONV_TAC(RAND_CONV EVAL)
+  \\ rw[wfpeg_Alt]);
+
+val wfpeg_Top = Q.store_thm("wfpeg_Top",
+  `wfpeg rePEG (nt (mkNT Top) I)`,
+  rw[Once wfpeg_cases] >- EVAL_TAC
+  \\ rw[wfpeg_Top_applied]);
+
+val wfG_rePEG = Q.store_thm("wfG_rePEG",
+  `wfG rePEG`,
+  simp[wfG_def,Gexprs_def,finite_mapTheory.IN_FRANGE,PULL_EXISTS,FDOM_rePEG]
+  \\ rw[] \\ pop_assum mp_tac
+  \\ TRY (
+    rename1`rePEG.rules ' (mkNT Atom)`
+    \\ CONV_TAC(LAND_CONV(RAND_CONV(RAND_CONV EVAL)))
+    \\ simp[subexprs_def]
+    \\ strip_tac \\ rpt BasicProvers.VAR_EQ_TAC
+    \\ rpt(rw[Once wfpeg_cases,wfpeg_Top,wfpeg_Alt,wfpeg_Concat,wfpeg_Star,wfpeg_Atom,wfpeg_BslashSpecial,wfpeg_CharSet]))
+  \\ CONV_TAC(LAND_CONV EVAL) \\ rw[]
+  \\ rpt(rw[Once wfpeg_cases,wfpeg_Top,wfpeg_Alt,wfpeg_Concat,wfpeg_Star,wfpeg_Atom]));
+
 
 (*
-open pegexecTheory
 val _ = computeLib.add_persistent_funs ["pegexec.peg_nt_thm"]
 
 val r = EVAL ``peg_exec rePEG rePEG.start "\\d" [] done failed``
